prepare for near-future merge into master by removing simple disk semantics and transformer, roll back Counter system

systems/Counter.v
@@ -1,8 +1,6 @@
 Require Import Verdi.Verdi.
 Require Import Verdi.HandlerMonad.
 
-Require Import Cheerios.Cheerios.
-
 Local Arguments update {_} {_} _ _ _ _ _ : simpl never.
 
 Set Implicit Arguments.
@@ -31,55 +29,38 @@ Definition Data := nat.
 
 Definition init_Data := 0.
 
-Definition Handler (S A : Type) := GenHandler (Name * Msg) S Output A.
+Definition Handler (S : Type) := GenHandler (Name * Msg) S Output unit.
 
-Definition disk := IOStreamWriter.wire.
-
-Definition snapshot : Handler Data disk :=
-  s <- get ;; ret (serialize_top (serialize s)).
-
-Definition reboot (s : IOStreamWriter.wire) : option Data :=
-  deserialize_top deserialize s.
-
-
-(* Definition keep_disk : Handler Data := *)
-Definition PrimaryNetHandler (m : Msg) : Handler Data unit :=
+Definition PrimaryNetHandler (m : Msg) : Handler Data :=
   match m with
   | ack => write_output inc_executed
   | _ => nop
   end.
 
-Definition PrimaryInputHandler (i : Input) : Handler Data unit :=
+Definition PrimaryInputHandler (i : Input) : Handler Data :=
   match i with
   | request_inc => modify S ;; send (backup, inc)
   end.
 
-Definition BackupNetHandler (m : Msg) : Handler Data unit :=
+Definition BackupNetHandler (m : Msg) : Handler Data :=
   match m with
   | inc => modify S ;; send (primary, ack)
   | _ => nop
   end.
 
-Definition BackupInputHandler (i : Input) : Handler Data unit := nop.
+Definition BackupInputHandler (i : Input) : Handler Data := nop.
 
-Definition NetHandler' (me : Name) (m : Msg) : Handler Data unit :=
+Definition NetHandler (me : Name) (m : Msg) : Handler Data :=
   match me with
   | primary => PrimaryNetHandler m
   | backup => BackupNetHandler m
   end.
 
-Definition NetHandler (me : Name) (m : Msg) : Handler Data disk :=
-  NetHandler' me m ;;
-              snapshot.
-
-Definition InputHandler' (me : Name) (i : Input) : Handler Data unit :=
+Definition InputHandler (me : Name) (i : Input) : Handler Data :=
   match me with
   | primary => PrimaryInputHandler i
   | backup => BackupInputHandler i
   end.
-
-Definition InputHandler (me : Name) (i : Input) : Handler Data disk :=
-  InputHandler' me i;; snapshot.
 
 Instance Counter_BaseParams : BaseParams :=
   {
@@ -100,69 +81,63 @@ Proof.
   repeat constructor; simpl; intuition discriminate.
 Qed.
 
-Instance Counter_DiskMultiParams : DiskMultiParams Counter_BaseParams :=
+Instance Counter_MultiParams : MultiParams Counter_BaseParams :=
   {
-    d_name := Name;
-    d_name_eq_dec := Name_eq_dec;
-    d_msg := Msg;
-    d_msg_eq_dec := Msg_eq_dec;
-    d_nodes := Nodes;
-    d_all_names_nodes := all_Names_Nodes;
-    d_no_dup_nodes := NoDup_Nodes;
-    d_init_handlers := fun _ => init_Data;
-    d_init_disk := fun _ => (serialize_top (serialize init_Data));
-    d_net_handlers := fun dst src msg s => runGenHandler s (NetHandler dst msg);
-    d_input_handlers := fun nm i s => runGenHandler s (InputHandler nm i)
+    name := Name;
+    name_eq_dec := Name_eq_dec;
+    msg := Msg;
+    msg_eq_dec := Msg_eq_dec;
+    nodes := Nodes;
+    all_names_nodes := all_Names_Nodes;
+    no_dup_nodes := NoDup_Nodes;
+    init_handlers := fun _ => init_Data;
+    net_handlers := fun dst src msg s =>
+                      runGenHandler_ignore s (NetHandler dst msg);
+    input_handlers := fun nm i s =>
+                      runGenHandler_ignore s (InputHandler nm i)
   }.
 
-Instance Counter_FailureParams : DiskFailureParams Counter_DiskMultiParams :=
-  {
-    d_reboot :=
-      fun _ s =>
-        match deserialize_top deserialize s with
-        | Some d => d
-        | None => init_Data
-        end
-  }.
 
 Lemma net_handlers_NetHandler :
-  forall h src m d os d' ms dsk,
-    d_net_handlers h src m d = (dsk, os, d', ms) ->
-    NetHandler h m d = (dsk, os, d', ms).
+  forall h src m d os d' ms,
+    net_handlers h src m d = (os, d', ms) ->
+    NetHandler h m d = (tt, os, d', ms).
 Proof.
   intros.
   simpl in *.
   monad_unfold.
   repeat break_let.
-  auto.
+  find_inversion.
+  destruct u. auto.
 Qed.
 
 Lemma input_handlers_InputHandlers :
-  forall h i d os d' ms dsk,
-    d_input_handlers h i d = (dsk, os, d', ms) ->
-    InputHandler h i d = (dsk, os, d', ms).
+  forall h i d os d' ms,
+    input_handlers h i d = (os, d', ms) ->
+    InputHandler h i d = (tt, os, d', ms).
 Proof.
   intros.
   simpl in *.
   monad_unfold.
   repeat break_let.
-  auto.
+  find_inversion.
+  destruct u. auto.
 Qed.
 
 Lemma PrimaryNetHandler_no_msgs :
   forall m d ms d' o u,
-    (PrimaryNetHandler m;; snapshot)  d = (u, o, d', ms) ->
+    PrimaryNetHandler m d = (u, o, d', ms) ->
     ms = [].
 Proof.
-  unfold PrimaryNetHandler, snapshot.
+  unfold PrimaryNetHandler.
   intros. monad_unfold.
-  repeat break_match; repeat find_inversion; auto.
+  break_match; find_inversion; auto.
 Qed.
 
-Definition inc_in_flight_to_backup (l : list d_packet) : nat :=
+Definition inc_in_flight_to_backup (l : list packet) : nat :=
   length (filterMap
-            (fun p => if d_msg_eq_dec (d_pBody p) inc
-                   then if d_name_eq_dec (d_pDst p) backup
+            (fun p => if msg_eq_dec (pBody p) inc
+                   then if name_eq_dec (pDst p) backup
                         then Some tt else None
                    else None)
             l).
@@ -180,7 +155,7 @@ Qed.
 
 Lemma inc_in_flight_to_backup_cons_primary_dst :
   forall p,
-    d_pDst p = primary ->
+    pDst p = primary ->
     inc_in_flight_to_backup [p] = 0.
 Proof.
   intros.
@@ -198,26 +173,26 @@ Qed.
 Lemma InputHandler_inc_in_flight_to_backup_preserved :
   forall h i d u o d' l,
     InputHandler h i d = (u, o, d', l) ->
-    d' = d + inc_in_flight_to_backup (d_send_packets h l).
+    d' = d + inc_in_flight_to_backup (send_packets h l).
 Proof.
-  unfold InputHandler, InputHandler', PrimaryInputHandler, BackupInputHandler, snapshot.
+  unfold InputHandler, PrimaryInputHandler, BackupInputHandler.
   simpl.
   intros.
   monad_unfold.
-  repeat break_match; repeat find_inversion; compute; auto.
+  repeat break_match; find_inversion; compute; auto.
   rewrite plus_comm. auto.
 Qed.
 
 Lemma NetHandler_inc_in_flight_to_backup_preserved :
   forall p d u o d' l,
-    NetHandler (d_pDst p) (d_pBody p) d = (u, o, d', l) ->
-    d' + inc_in_flight_to_backup (d_send_packets (d_pDst p) l) = d + inc_in_flight_to_backup [p].
+    NetHandler (pDst p) (pBody p) d = (u, o, d', l) ->
+    d' + inc_in_flight_to_backup (send_packets (pDst p) l) = d + inc_in_flight_to_backup [p].
 Proof.
-  unfold NetHandler, NetHandler', PrimaryNetHandler, BackupNetHandler.
+  unfold NetHandler, PrimaryNetHandler, BackupNetHandler.
   intros.
   monad_unfold.
   destruct p. simpl in *.
-  repeat break_match; repeat find_inversion; simpl; try rewrite inc_in_flight_to_backup_nil;
+  repeat break_match; find_inversion; simpl; try rewrite inc_in_flight_to_backup_nil;
   unfold Data in *; compute;
   auto with *.
 Qed.
@@ -227,9 +202,9 @@ Lemma InputHandler_backup_no_msgs :
     InputHandler backup i d = (u, o, d', l) ->
     l = [].
 Proof.
-  simpl. unfold InputHandler, InputHandler', BackupInputHandler.
+  simpl. unfold BackupInputHandler.
   intros.
-  unfold snapshot in *. monad_unfold.
+  monad_unfold.
   find_inversion.
   auto.
 Qed.
@@ -241,40 +216,32 @@ Proof.
   auto.
 Qed.
 
-
-
 Lemma backup_plus_network_eq_primary :
   forall net tr,
-    step_async_disk_star (params := Counter_DiskMultiParams)
-                         step_async_disk_init
-                         net tr -> 
-    nwdState net backup + inc_in_flight_to_backup (nwdPackets net) = nwdState net primary.
+    step_async_star (params := Counter_MultiParams) step_async_init net tr ->
+    nwState net backup + inc_in_flight_to_backup (nwPackets net) = nwState net primary.
 Proof.
   intros.
-  remember step_async_disk_init as y in *.
+  remember step_async_init as y in *.
   revert Heqy.
   induction H using refl_trans_1n_trace_n1_ind; intros; subst.
   - reflexivity.
   - concludes.
     match goal with
-    | [ H : step_async_disk _ _ _ |- _ ] => invc H
+    | [ H : step_async _ _ _ |- _ ] => invc H
     end; simpl.
     + find_apply_lem_hyp net_handlers_NetHandler.
       find_copy_apply_lem_hyp NetHandler_inc_in_flight_to_backup_preserved.
       repeat find_rewrite.
       rewrite cons_is_app in IHrefl_trans_1n_trace1.
       repeat rewrite inc_in_flight_to_backup_app in *.
-      destruct (d_pDst p) eqn:?;
+      destruct (pDst p) eqn:?;
                try rewrite update_same;
         try rewrite update_diff by congruence;
-        unfold d_send_packets in *; simpl in *.
+        unfold send_packets in *; simpl in *.
       * erewrite PrimaryNetHandler_no_msgs with (ms := l) in * by eauto.
-        simpl in *. rewrite inc_in_flight_to_backup_nil in *.
-        rewrite inc_in_flight_to_backup_cons_primary_dst in *;
-          (repeat rewrite <- plus_n_O in *);
-           simpl in *;
-           try rewrite H0;
-           assumption.
+        rewrite inc_in_flight_to_backup_cons_primary_dst in * by auto.
+        simpl in *. rewrite inc_in_flight_to_backup_nil in *. auto with *.
       * omega.
     + find_apply_lem_hyp input_handlers_InputHandlers.
       find_copy_apply_lem_hyp InputHandler_inc_in_flight_to_backup_preserved.
@@ -290,15 +257,15 @@ Qed.
 
 Theorem primary_ge_backup :
   forall net tr,
-    step_async_disk_star (params := Counter_DiskMultiParams) step_async_disk_init net tr ->
-    nwdState net backup <= nwdState net primary.
+    step_async_star (params := Counter_MultiParams) step_async_init net tr ->
+    nwState net backup <= nwState net primary.
 Proof.
   intros.
   apply backup_plus_network_eq_primary in H.
   auto with *.
 Qed.
 
-Definition trace_inputs (tr : list (d_name * (input + list output))) : nat :=
+Definition trace_inputs (tr : list (name * (input + list output))) : nat :=
   length (filterMap (fun e => match e with
                            | (primary, inl i) => Some i
                            | _ => None
@@ -313,7 +280,7 @@ Proof.
   rewrite app_length. auto.
 Qed.
 
-Definition trace_outputs (tr : list (d_name * (input + list output))) : nat :=
+Definition trace_outputs (tr : list (name * (input + list output))) : nat :=
   length (filterMap (fun e => match e with
                            | (primary, inr [o]) => Some o
                            | _ => None
@@ -329,10 +296,10 @@ Proof.
   rewrite app_length. auto.
 Qed.
 
-Definition ack_in_flight_to_primary (l : list d_packet) : nat :=
+Definition ack_in_flight_to_primary (l : list packet) : nat :=
   length (filterMap
-            (fun p => if d_msg_eq_dec (d_pBody p) ack
-                   then if d_name_eq_dec (d_pDst p) primary
+            (fun p => if msg_eq_dec (pBody p) ack
+                   then if name_eq_dec (pDst p) primary
                         then Some tt else None
                    else None)
             l).
@@ -349,7 +316,7 @@ Qed.
 
 Lemma ack_in_flight_to_primary_backup :
   forall p,
-    d_pDst p = backup ->
+    pDst p = backup ->
     ack_in_flight_to_primary [p] = 0.
 Proof.
   intros.
@@ -364,30 +331,30 @@ Lemma InputHandler_trace_preserved :
     InputHandler h i d = (u, o, d', l) ->
     trace_inputs [(h, inl i)] =
     trace_outputs [(h, inr o)] +
-    inc_in_flight_to_backup (d_send_packets h l) +
-    ack_in_flight_to_primary (d_send_packets h l).
+    inc_in_flight_to_backup (send_packets h l) +
+    ack_in_flight_to_primary (send_packets h l).
 Proof.
-  unfold InputHandler, InputHandler', snapshot, PrimaryInputHandler, BackupInputHandler.
+  unfold InputHandler, PrimaryInputHandler, BackupInputHandler.
   simpl.
   intros.
   monad_unfold.
-  repeat break_match; repeat find_inversion; compute; auto.
+  repeat break_match; find_inversion; compute; auto.
 Qed.
 
 Lemma NetHandler_trace_preserved :
   forall p d u o d' l,
-    NetHandler (d_pDst p) (d_pBody p) d = (u, o, d', l) ->
+    NetHandler (pDst p) (pBody p) d = (u, o, d', l) ->
     inc_in_flight_to_backup [p] +
     ack_in_flight_to_primary [p] =
-    trace_outputs [((d_pDst p), inr o)] +
-    inc_in_flight_to_backup (d_send_packets (d_pDst p) l) +
-    ack_in_flight_to_primary (d_send_packets (d_pDst p) l).
+    trace_outputs [((pDst p), inr o)] +
+    inc_in_flight_to_backup (send_packets (pDst p) l) +
+    ack_in_flight_to_primary (send_packets (pDst p) l).
 Proof.
-  unfold NetHandler, NetHandler', snapshot, PrimaryNetHandler, BackupNetHandler.
+  unfold NetHandler, PrimaryNetHandler, BackupNetHandler.
   intros.
   monad_unfold.
   destruct p. simpl in *.
-  repeat break_match; repeat find_inversion; simpl; try rewrite inc_in_flight_to_backup_nil;
+  repeat break_match; find_inversion; simpl; try rewrite inc_in_flight_to_backup_nil;
   unfold Data in *; compute;
   auto with *.
 Qed.
@@ -419,19 +386,19 @@ Qed.
 
 Lemma inputs_eq_outputs_plus_inc_plus_ack :
   forall net tr,
-    step_async_disk_star (params := Counter_DiskMultiParams) step_async_disk_init net tr ->
+    step_async_star (params := Counter_MultiParams) step_async_init net tr ->
     trace_inputs tr = trace_outputs tr +
-                      inc_in_flight_to_backup (nwdPackets net) +
-                      ack_in_flight_to_primary (nwdPackets net).
+                      inc_in_flight_to_backup (nwPackets net) +
+                      ack_in_flight_to_primary (nwPackets net).
 Proof.
   intros.
-  remember step_async_disk_init as y in *.
+  remember step_async_init as y in *.
   revert Heqy.
   induction H using refl_trans_1n_trace_n1_ind; intros; subst.
   - reflexivity.
   - concludes.
     match goal with
-    | [ H : step_async_disk _ _ _ |- _ ] => invc H
+    | [ H : step_async _ _ _ |- _ ] => invc H
     end; simpl.
     + find_apply_lem_hyp net_handlers_NetHandler.
       repeat find_rewrite.
@@ -441,7 +408,7 @@ Proof.
       repeat rewrite inc_in_flight_to_backup_app in *.
       repeat rewrite ack_in_flight_to_primary_app in *.
       find_apply_lem_hyp NetHandler_trace_preserved.
-      destruct (d_pDst p) eqn:?.
+      destruct (pDst p) eqn:?.
       * erewrite inc_in_flight_to_backup_cons_primary_dst in * by eauto.
         rewrite trace_inputs_output in *. simpl in  *. omega.
       * rewrite ack_in_flight_to_primary_backup in * by auto.
@@ -461,99 +428,10 @@ Qed.
 
 Theorem inputs_ge_outputs :
   forall net tr,
-    step_async_disk_star (params := Counter_DiskMultiParams) step_async_disk_init net tr ->
+    step_async_star (params := Counter_MultiParams) step_async_init net tr ->
     trace_outputs tr <= trace_inputs tr.
 Proof.
   intros.
   apply inputs_eq_outputs_plus_inc_plus_ack in H.
   omega.
-Qed.
-
-Theorem net_handlers_reboot : forall node net p out d l dsk,
-    d_net_handlers node
-                   (d_pSrc p) (d_pBody p)
-                   (nwdState net node) = (dsk, out, d, l) ->
-      reboot (update Name_eq_dec (nwdDisk net) node dsk node) =
-  Some (update Name_eq_dec (nwdState net) node d node).
-Proof.
-  intros.
-  simpl in *.
-  destruct node;
-    unfold runGenHandler, NetHandler, NetHandler', PrimaryNetHandler, BackupNetHandler, snapshot in *;
-    monad_unfold;
-    repeat break_match;
-    repeat find_inversion;
-    apply serialize_deserialize_top_id.
-Qed.
-
-Theorem input_handlers_reboot : forall node net inp out d l dsk,
-    d_input_handlers node
-                     inp
-                   (nwdState net node) = (dsk, out, d, l) ->
-      reboot (update Name_eq_dec (nwdDisk net) node dsk node) =
-  Some (update Name_eq_dec (nwdState net) node d node).
-Proof.
-  intros.
-  simpl in *.
-  destruct node;
-    unfold runGenHandler, InputHandler, InputHandler', PrimaryInputHandler, BackupInputHandler, snapshot in *;
-    monad_unfold;
-    repeat break_match;
-    repeat find_inversion;
-    apply serialize_deserialize_top_id.
-Qed.
-
-Theorem disk_follows_local_state: forall net tr node,
-    step_async_disk_star (params := Counter_DiskMultiParams) step_async_disk_init net tr ->
-    reboot (nwdDisk net node) = Some (nwdState net node).
-Proof.
-  intros.
-  remember step_async_disk_init as y in *.
-  revert Heqy.
-  induction H using refl_trans_1n_trace_n1_ind; intros; subst.
-  - simpl.
-    unfold init_Data.
-    apply serialize_deserialize_top_id.
-  - concludes.
-    match goal with
-    | [ H : step_async_disk _ _ _ |- _ ] => invc H
-    end; simpl.
-    + destruct node, (d_pDst p).
-      * match goal with
-        | [H : d_net_handlers ?node _ _ _ = _ |- _] =>
-          apply (net_handlers_reboot node _ _ H)
-        end.
-      * rewrite update_diff.
-        -- rewrite update_diff.
-           ++ assumption.
-           ++ discriminate.
-        -- discriminate.
-      * rewrite update_diff.
-        -- rewrite update_diff.
-           ++ assumption.
-           ++ discriminate.
-        -- discriminate.
-      * match goal with
-        | [H : d_net_handlers ?node _ _ _ = _ |- _] =>
-          apply (net_handlers_reboot node _ _ H)
-        end.
-    + destruct node, h.
-      * match goal with
-        | [H : d_input_handlers ?node _ _ = _ |- _] =>
-          apply (input_handlers_reboot node _ _ H)
-        end.
-      * rewrite update_diff.
-        -- rewrite update_diff.
-           ++ assumption.
-           ++ discriminate.
-        -- discriminate.
-      * rewrite update_diff.
-        -- rewrite update_diff.
-           ++ assumption.
-           ++ discriminate.
-        -- discriminate.
-      * match goal with
-        | [H : d_input_handlers ?node _ _ = _ |- _] =>
-          apply (input_handlers_reboot node _ _ H)
-        end.
 Qed.
